\section{Toy model}

A quick derivation of how the center of mass changes when we add a parabolic term to the 2DEG Landau Level system.
Start with the Landau level Hamiltonian with a perpendicular magentic field and additional parabolic term

\begin{equation}
  \ham = \dfrac{p_x^2}{2m} + \dfrac{1}{2m} {\left(p_y + eBx \right)}^2 + \dfrac{e^2 B_1^2}{2m} x^2
\end{equation}
We want to utilize the Laughlin pump argument.
we imagine the y-axis is wrapped around to make a cylinder with circumference $L$ which makes $k=\tfrac{2\pi m}{L}$.
Then add in a flux term $\Phi(t)$ along the x-axis, the Hamiltonian becomes

\begin{equation}
  \ham = \dfrac{p_x^2}{2m} + \dfrac{1}{2m} {\left(qBx + q\Phi + \hbar k \right)}^2 + \dfrac{q^2 B_1^2}{2m} x^2
\end{equation}
Performing a shift in coordinates of $x' = x + \tfrac{\Phi}{BL} + \tfrac{\hbar k}{qB}$

\begin{align}
  \ham &= \dfrac{p_x^2}{2m} + \dfrac{q^2B^2x'^2}{2m} + \dfrac{q^2 B_1^2}{2m} {\left( x' - \dfrac{\Phi}{BL} - \dfrac{\hbar k}{qB} \right)}^2 \nonumber \\
  &= \dfrac{p_{x'}^2}{2m} + \dfrac{q^2B^2x'^2}{2m} + \dfrac{q^2 B_1^2}{2m} x'^2 - 2\dfrac{q^2 B_1^2}{2m} \Phi'(k)x' + \dfrac{q^2 B_1^2}{2m} \Phi'^2(k) \nonumber \\
  &= \dfrac{p_{x'}^2}{2m} + \dfrac{q^2B_2^2}{2m} \left( x'^2  - \dfrac{2B_1^2\Phi'(k)x'}{B_2^2} + \dfrac{B_1^4 \Phi'^2(k)}{B_2^4} \left) -\dfrac{q^2B_1^4\Phi'^2(k)}{2mB_2^2} + \dfrac{q^2 B_1^2}{2m} \Phi'^2 \nonumber \\
  &= \dfrac{p_{x'}^2}{2m} + \dfrac{q^2B_2^2}{2m} \left( x'  - \dfrac{B_1^2\Phi'(k)x'}{B_2^2} \left)^2 - \dfrac{B_1^2 \Phi'^2(k)}{B_2^2} (q^2 B_1^2 - q^2B_2^2) \nonumber \\
  &= \dfrac{p_{x''}^2}{2m} + \dfrac{q^2B_2^2x''^2}{2m} + \dfrac{B^2 B_1^2 \Phi'^2(k) }{2mB_2^2}
\end{align}
where

\begin{align}
  x'' &= x'- \tfrac{B_1^2\Phi'(k)}{B_2^2} \nonumber \\
  &= x + \Phi'(k) - \Phi'(k)\dfrac{B_1^2}{B_2^2} \nonumber \\
  &= x + \Phi'(k)\dfrac{B^2}{B_2^2} \nonumber \\
  &= x + \left(\dfrac{\Phi}{BL} + \dfrac{\hbar k}{eB} \right) \dfrac{B^2}{B_2^2} \nonumber \\
  &= x + \left(kL + \dfrac{2\pi\Phi}{\Phi_0}\right) \dfrac{\hbar B}{eL B_2^2} \nonumber \\
  &= x + \left(m + \dfrac{\Phi}{\Phi_0} \right) \dfrac{B \Phi_0}{L B_2^2}
\end{align}
and $ B_2^2 = B^2 + B_1^2$.
If we include a periodic potential in the y-axis, $b\cos(Ky)$, the Hamiltonian becomes

\begin{align}
  \ham = \dfrac{p_{x''}^2}{2m} + \dfrac{q^2B_2^2x''^2}{2m} + \dfrac{B^2 B_1^2 \Phi'^2(p_y) }{2mB_2^2} + b\cos(Ky)
\end{align}
Using Bloch theorem we state

\begin{align}
  \Psi_k (x,y) &= e^{ika_y}\Psi(x,y+a_y) \nonumber \\
  \Psi_k (x,y) &= e^{iky} u_k(x,y) \nonumber \\
  u_k(x,y) &= u_k(x,y+a_y) \nonumber \\
  u_k(x,y) &= \sum_l u_{k,l}(x) e^{ilKy} \nonumber \\
  \Psi_k (x,y) &= \sum_l u_{k,l}(x) e^{i(lK+k)y} = \sum_m u_{k,l}(x) e^{ik'y}.
\end{align}
Acting the Hamiltonian on the ansatz wavefunction gives

\begin{align}
  \ham\Psi_k(x,y) &= \sum_l \left[ \left( \dfrac{p_{x''}^2}{2m} + \dfrac{q^2B_2^2x''^2}{2m} + \dfrac{B^2 B_1^2 \Phi'^2(k') }{2mB_2^2}\right) u_{k,l} + \dfrac{b}{2} \left(u_{k,l+1} + u_{k,l-1} \right) \right] e^{ik'y} \nonumber \\
  &= E_n(k')\Psi_k(x,y) + \sum_l \dfrac{b}{2} \left( u_{k,l+1} + u_{k,l-1} \right) e^{ik'y}
\end{align}
